backends/lean/Aeneas/Tactic/Solver/BvTac/BvTac.lean
@@ -23,7 +23,7 @@ partial def getn : TacticM Expr := do
   let mgoal ← getMainGoal
   let goalTy ← instantiateMVars (← mgoal.getType)
   let raiseError : TacticM Expr :=
-    throwError "Could not infer the bitwidth to use by from the goal, please provide it explicitly with the syntax: `bv_tac n`"
+    throwError "Could not infer the bitwidth to use by from the goal, please provide it explicitly with the syntax: `toBitVec_tac n`"
   let fromBitVecTy (ty : Expr) : TacticM Expr :=
     ty.consumeMData.withApp fun f args => do
     trace[BvTac] "fromBitVecTy: {f}, {args}"
@@ -76,37 +76,37 @@ partial def bvTacPreprocess (config : Config) (n : Option Expr): TacticM Unit :=
   -- The simpAll may have solved the goal, so we need to be careful
   Utils.allGoals do trace[BvTac] "Goal after `simp_all`: {← getMainGoal}"
 
-elab "bv_tac_preprocess" config:Parser.Tactic.optConfig n:(colGt term)? : tactic => do
+elab "toBitVec_tac_preprocess" config:Parser.Tactic.optConfig n:(colGt term)? : tactic => do
   bvTacPreprocess (← elabConfig config) (← optElabTerm n)
 
 open Lean.Elab.Tactic.BVDecide.Frontend Lean.Elab in
-/-- `bv_tac n` solves goals about bit-vectors.
+/-- `toBitVec_tac n` solves goals about bit-vectors.
 
-**Usage**: `bv_tac n` where `n` is the bitwidth to use for the bit-vectors.
+**Usage**: `toBitVec_tac n` where `n` is the bitwidth to use for the bit-vectors.
 The bitwidth `n` can sometimes be inferred automatically from the goal in which case
 it can be omitted.
 
 **Preprocessing**:
-`bv_tac` first preprocesses the goal (essentially by using `bvify`) to lift inequalities
-so that they use bit-vectors rather than `ℕ` or `ℤ`, before calling `bv_decide`.
+`toBitVec_tac` first preprocesses the goal (essentially by using `bvify`) to lift inequalities
+so that they use bit-vectors rather than `ℕ` or `ℤ`, before calling `toBitVec_decide`.
 This can sometimes fail as lifting those inequalities requires solving arithmetic proof
-obligations. For this reason, when `bv_tac` fails, we advise looking carefully at the goal
+obligations. For this reason, when `toBitVec_tac` fails, we advise looking carefully at the goal
 to check if all the expected inequalities have been lifted to bit-vectors. If some could not
 be lifted, one can try lifting them manually - see the documentation of `bvify` for some tips
 and tricks.
 
 **Debugging**:
-Calling `bv_tac n` is (roughly) equivalent to: `bv_tac_preprocess n; bv_decide`,
-which is itself roughly equivalent to: `bvify n at *; simp_all only; bv_decide`.
+Calling `toBitVec_tac n` is (roughly) equivalent to: `toBitVec_tac_preprocess n; toBitVec_decide`,
+which is itself roughly equivalent to: `bvify n at *; simp_all only; toBitVec_decide`.
 
-Note that it often happens that `bv_tac` fails because `bvify` could not
-lift some assumptions to the subset `bv_decide` can reason about. For this
-reason, it is often useful to inspect the goal after calling `bvify` (or `bv_tac_preprocess`).
+Note that it often happens that `toBitVec_tac` fails because `bvify` could not
+lift some assumptions to the subset `toBitVec_decide` can reason about. For this
+reason, it is often useful to inspect the goal after calling `bvify` (or `toBitVec_tac_preprocess`).
 Typically problematic terms are applications of `BitVec.ofNat` to complex expressions
-(for instance, `bv_decide` can generally not reason about `BitVec.ofNat n (a + b)`, which we
+(for instance, `toBitVec_decide` can generally not reason about `BitVec.ofNat n (a + b)`, which we
 want to simplify to `BitVec.ofNat n a + BitVec.ofNat n b`).
 -/
-elab "bv_tac" config:Parser.Tactic.optConfig n:(colGt term)? : tactic =>
+elab "toBitVec_tac" config:Parser.Tactic.optConfig n:(colGt term)? : tactic =>
   withMainContext do
   Tactic.focus do
   -- Preprocess
@@ -115,7 +115,7 @@ elab "bv_tac" config:Parser.Tactic.optConfig n:(colGt term)? : tactic =>
   bvTacPreprocess config (← optElabTerm n)
   -- The preprocessing step may have proven the goal
   Utils.allGoals do
-  -- Call bv_decide
+  -- Call toBitVec_decide
   IO.FS.withTempFile fun _ lratFile => do
     let config := config.toBVDecideConfig
     let cfg ← BVDecide.Frontend.TacticContext.new lratFile config
@@ -127,28 +127,28 @@ elab "bv_tac" config:Parser.Tactic.optConfig n:(colGt term)? : tactic =>
 -/
 open Std
 
-example (x y : U8) (h : x.val ≤ y.val) : x.bv ≤ y.bv := by
-  bv_tac
+example (x y : U8) (h : x.val ≤ y.val) : x.toBitVec ≤ y.toBitVec := by
+  toBitVec_tac
 
-example (x : U32) (h : x.val < 3329) : x.bv % 3329#32 = x.bv := by
-  bv_tac
+example (x : U32) (h : x.val < 3329) : x.toBitVec % 3329#32 = x.toBitVec := by
+  toBitVec_tac
 
 /- Checking parsing -/
-example (x : U32) (h : x.val < 3329) : x.bv % 3329#32 = x.bv ∧ True := by
+example (x : U32) (h : x.val < 3329) : x.toBitVec % 3329#32 = x.toBitVec ∧ True := by
   constructor
-  bv_tac
+  toBitVec_tac
   simp
 
 /- Checking parsing -/
-example (x : U32) (h : x.val < 3329) : x.bv % 3329#32 = x.bv ∧ True := by
+example (x : U32) (h : x.val < 3329) : x.toBitVec % 3329#32 = x.toBitVec ∧ True := by
   constructor
-  bv_tac 32
+  toBitVec_tac 32
   simp
 
 /- Checking parsing -/
-example (x : U32) (h : x.val < 3329) : x.bv % 3329#32 = x.bv ∧ True := by
+example (x : U32) (h : x.val < 3329) : x.toBitVec % 3329#32 = x.toBitVec ∧ True := by
   constructor
-  bv_tac 32; simp
+  toBitVec_tac 32; simp
 
 example
   (a : U32)
@@ -156,15 +156,15 @@ example
   (ha : a.val < 3329)
   (hb : b.val < 3329)
   (c1 : U32)
-  (_ : c1.bv = a.bv + b.bv)
+  (_ : c1.toBitVec = a.toBitVec + b.toBitVec)
   (c2 : U32)
   (hc2 : c2 = core.num.U32.wrapping_sub c1 3329#u32)
   (c3 : U32)
-  (hc3 : c3.bv = c2.bv >>> 16#i32.toNat)
+  (hc3 : c3.toBitVec = c2.toBitVec >>> 16#i32.toNat)
   (_ : ¬c3 = 0#u32) :
   c3 = 65535#u32
   := by
-  bv_tac
+  toBitVec_tac
 
 example
   (a : U32)
@@ -172,14 +172,14 @@ example
   (ha : a.val < 3329)
   (hb : b.val < 3329)
   (c1 : U32)
-  (_ : c1.bv = a.bv + b.bv)
+  (_ : c1.toBitVec = a.toBitVec + b.toBitVec)
   (c2 : U32)
   (_ : c2 = core.num.U32.wrapping_sub c1 3329#u32)
   (c3 : U32)
-  (_ : c3.bv = c2.bv >>> 16#i32.toNat) :
-  (c1.bv - 3329#32 + (3329#32 &&& c3.bv)) % 3329#32 = (a.bv + b.bv) % 3329#32
+  (_ : c3.toBitVec = c2.toBitVec >>> 16#i32.toNat) :
+  (c1.toBitVec - 3329#32 + (3329#32 &&& c3.toBitVec)) % 3329#32 = (a.toBitVec + b.toBitVec) % 3329#32
   := by
-  bv_tac
+  toBitVec_tac
 
 example
   (a : U32)
@@ -187,12 +187,12 @@ example
   (c1 : U32)
   (hc1 : c1 = core.num.U32.wrapping_sub a b)
   (c2 : U32)
-  (hc2 : c2.bv = c1.bv >>> 16#i32.toNat)
+  (hc2 : c2.toBitVec = c1.toBitVec >>> 16#i32.toNat)
   (h : (↑a : ℕ) < 6658 ∧ (↑b : ℕ) = 3329)
   (_ : ¬c2 = 0#u32) :
   c2 = 65535#u32
   := by
-  bv_tac
+  toBitVec_tac
 
 example
   (a : U32)
@@ -203,15 +203,15 @@ example
   (c1 : U32)
   (hc1 : c1 = core.num.U32.wrapping_sub a b)
   (c2 : U32)
-  (hc2 : c2.bv = c1.bv >>> 16)
+  (hc2 : c2.toBitVec = c1.toBitVec >>> 16)
   (c3 : U32)
   (hc3_1 : (↑c3 : ℕ) = (↑(3329#u32 &&& c2) : ℕ))
-  (_ : c3.bv = 3329#32 &&& c2.bv)
+  (_ : c3.toBitVec = 3329#32 &&& c2.toBitVec)
   (c4 : U32)
   (hc3 : c4 = core.num.U32.wrapping_add c1 c3) :
-  c4.bv % 3329#32 = (a.bv + 3329#32 - b.bv) % 3329#32 ∧ c4.bv < 3329#32
+  c4.toBitVec % 3329#32 = (a.toBitVec + 3329#32 - b.toBitVec) % 3329#32 ∧ c4.toBitVec < 3329#32
   := by
-  bv_tac
+  toBitVec_tac
 
 example
   (a : U32)
@@ -220,14 +220,14 @@ example
   (hb : (↑b : ℕ) < 3329)
   (c1 : U32)
   (hc1 : (↑c1 : ℕ) = (↑a : ℕ) + (↑b : ℕ))
-  (_ : c1.bv = a.bv + b.bv)
+  (_ : c1.toBitVec = a.toBitVec + b.toBitVec)
   (c2 : U32)
   (hc2 : c2 = core.num.U32.wrapping_sub c1 3329#u32)
   (c3 : U32)
-  (hc3 : c3.bv = c2.bv >>> 16)
+  (hc3 : c3.toBitVec = c2.toBitVec >>> 16)
   (h : ¬c3 = 0#u32) :
   c3 = 65535#u32
-  := by bv_tac
+  := by toBitVec_tac
 
 example
   (a : U32)
@@ -236,10 +236,10 @@ example
   (c1 : U32)
   (hc1 : c1 = core.num.U32.wrapping_sub a b)
   (c2 : U32)
-  (hc2 : c2.bv = c1.bv >>> 16) :
+  (hc2 : c2.toBitVec = c1.toBitVec >>> 16) :
   (decide (c2 = 0#u32) || decide (c2 = 65535#u32)) = true
   := by
-  bv_tac
+  toBitVec_tac
 
 example
   (a : U32)
@@ -248,14 +248,14 @@ example
   (c1 : U32)
   (hc1 : c1 = core.num.U32.wrapping_sub a b)
   (c2 : U32)
-  (hc2 : c2.bv = c1.bv >>> 16)
+  (hc2 : c2.toBitVec = c1.toBitVec >>> 16)
   (c3 : U32)
   (hc3_1 : c3.val = (3329#u32 &&& c2).val)
-  (_ : c3.bv = 3329#32 &&& c2.bv)
+  (_ : c3.toBitVec = 3329#32 &&& c2.toBitVec)
   (c4 : U32)
   (hc3 : c4 = core.num.U32.wrapping_add c1 c3) :
   (c4.val : ZMod 3329) = (a.val : ZMod 3329) - (b.val : ZMod 3329) ∧ c4.val < 3329
   := by
-  bv_tac 32
+  toBitVec_tac 32
 
 end Aeneas.BvTac
